# baseURI: http://w3id.org/idpo
# imports: http://purl.org/dc/elements/1.1/
# imports: http://www.w3.org/ns/shacl#
# imports: https://standards.iso.org/iso/21597/-1/ed-1/en/Container.rdf
# prefix: idpo

@prefix bpmn: <http://www.omg.org/spec/BPMN/20100524/MODEL#> .
@prefix ct: <https://standards.iso.org/iso/21597/-1/ed-1/en/Container#> .
@prefix dc: <http://purl.org/dc/elements/1.1/> .
@prefix dcterms: <http://purl.org/dc/terms/> .
@prefix idpo: <http://w3id.org/idpo#> .
@prefix owl: <http://www.w3.org/2002/07/owl#> .
@prefix prov: <http://www.w3.org/ns/prov#> .
@prefix rdf: <http://www.w3.org/1999/02/22-rdf-syntax-ns#> .
@prefix rdfs: <http://www.w3.org/2000/01/rdf-schema#> .
@prefix sdo: <https://schema.org/> .
@prefix sh: <http://www.w3.org/ns/shacl#> .
@prefix skos: <http://www.w3.org/2004/02/skos/core#> .
@prefix vann: <http://purl.org/vocab/vann/> .
@prefix voaf: <http://purl.org/vocommons/voaf#> .
@prefix xsd: <http://www.w3.org/2001/XMLSchema#> .

<http://w3id.org/idpo>
  rdf:type voaf:Vocabulary ;
  rdf:type owl:Ontology ;
  dcterms:created "2020-03-30"^^xsd:date ;
  dcterms:creator [
      rdf:type sdo:Person ;
      sdo:email <mailto:philipp.hagedorn-n6v@rub.de> ;
      sdo:identifier <https://orcid.org/0000-0002-6249-243X> ;
      sdo:memberOf [
          sdo:identifier <https://www.inf.bi.ruhr-uni-bochum.de/iib/lehrstuhl/mitarbeiter/philipp_hagedorn.html.en> ;
          sdo:name "Ruhr University Bochum" ;
        ] ;
      sdo:name "Philipp Hagedorn" ;
    ] ;
  dcterms:description "The Information Delivery Processes Ontology (IDPO) Ontology is defined for modeling information delivery in the construction planning based on BPMN processes and the PROV-Ontology. It provides SHACL templates for validating information requirements and delivery specifications." ;
  dcterms:license <https://creativecommons.org/licenses/by/4.0/> ;
  dcterms:modified "2023-02-20"^^xsd:date ;
  dcterms:publisher [
      rdf:type sdo:Organization ;
      rdf:type sdo:ResearchOrganization ;
      sdo:identifier <https://www.inf.bi.rub.de> ;
      sdo:name "Chair of Computing in Engineering, Ruhr University Bochum" ;
      sdo:parentOrganization [
          rdf:type sdo:Organization ;
          rdf:type sdo:ResearchOrganization ;
          sdo:name "Ruhr University Bochum, Germany" ;
        ] ;
    ] ;
  dcterms:source "https://git.inf.bi.ruhr-uni-bochum.de/semweb-ontology/idpo/" ;
  dcterms:title "Information Delivery Processes Ontology (IDPO)" ;
  vann:preferredNamespacePrefix "idpo" ;
  vann:preferredNamespaceUri idpo: ;
  owl:imports dc: ;
  owl:imports sh: ;
  owl:imports <https://standards.iso.org/iso/21597/-1/ed-1/en/Container.rdf> ;
  owl:versionInfo "v0.2" ;
  sh:declare idpo:PrefixDeclaration ;
  sh:declare bpmn:PrefixDeclaration ;
.
idpo:Actor
  rdf:type rdfs:Class ;
  idpo:isMemberOf idpo:Project ;
  rdfs:comment "ISO 19650-1 3.2.1 actor: person, organization or organizational unit involved in a construction process" ;
  rdfs:isDefinedBy <https://www.iso.org/standard/68078.html> ;
  rdfs:label "Actor" ;
  rdfs:subClassOf prov:Agent ;
  rdfs:subClassOf ct:Party ;
.
idpo:AppointedParty
  rdf:type rdfs:Class ;
  rdfs:comment "ISO 19650-1 3.2.3 appointed party: provider of information (3.3.1) concerning works, goods or services. Is equivalent to idpo:InformationProvider." ;
  rdfs:isDefinedBy <https://www.iso.org/standard/68078.html> ;
  rdfs:label "AppointedParty" ;
  rdfs:subClassOf idpo:Actor ;
  rdfs:subClassOf [
      rdf:type owl:Restriction ;
      owl:minCardinality "1"^^xsd:nonNegativeInteger ;
      owl:onProperty idpo:isAppointedForDelivery ;
    ] ;
  owl:equivalentClass idpo:InformationProvider ;
.
idpo:AppointingParty
  rdf:type rdfs:Class ;
  rdfs:comment "ISO 19650-1 3.2.4 appointing party: receiver of information (3.3.1) concerning works, goods or services from a lead appointed party (3.2.3). Is equivalent to idpo:InformationReceiver." ;
  rdfs:isDefinedBy <https://www.iso.org/standard/68078.html> ;
  rdfs:label "AppointingParty" ;
  rdfs:subClassOf idpo:Actor ;
  rdfs:subClassOf [
      rdf:type owl:Restriction ;
      owl:minCardinality "1"^^xsd:nonNegativeInteger ;
      owl:onProperty idpo:appointsUsage ;
    ] ;
  rdfs:subClassOf [
      rdf:type owl:Restriction ;
      owl:minCardinality "1"^^xsd:nonNegativeInteger ;
      owl:onProperty idpo:defines ;
    ] ;
  owl:equivalentClass idpo:InformationReceiver ;
.
idpo:ExchangeInformationRequirement
  rdf:type owl:Class ;
  rdfs:comment "ISO 19650-1 3.3.6 exchange information requirements (EIR): information requirements in relation to an appointment" ;
  rdfs:isDefinedBy <https://www.iso.org/standard/68078.html> ;
  rdfs:label "ExchangeInformationRequirement" ;
  rdfs:subClassOf owl:Thing ;
  rdfs:subClassOf [
      rdf:type owl:Restriction ;
      owl:cardinality "1"^^xsd:nonNegativeInteger ;
      owl:onProperty idpo:dueDate ;
    ] ;
  rdfs:subClassOf [
      rdf:type owl:Restriction ;
      owl:cardinality "1"^^xsd:nonNegativeInteger ;
      owl:onProperty idpo:priority ;
    ] ;
  rdfs:subClassOf [
      rdf:type owl:Restriction ;
      owl:cardinality "1"^^xsd:nonNegativeInteger ;
      owl:onProperty idpo:suitability ;
    ] ;
  rdfs:subClassOf [
      rdf:type owl:Restriction ;
      owl:minCardinality "1"^^xsd:nonNegativeInteger ;
      owl:onProperty idpo:hasInformationConstraint ;
    ] ;
.
idpo:InformationContainer
  rdf:type owl:Class ;
  rdfs:comment "ISO 19650-1 3.3.12 information container: named persistent set of information retrievable from within a file, system or application storage hierarchy. This class is used to represent a set of data summarized as an information container. Information containers can be generated and used. Instances of this class can be derived from bpmn2:DataObject individuals. This class is a subClass of prov:Entity which allows to associate additional provenance information. It is equivalent to the ct:ContainerDescription class from ICDD." ;
  rdfs:isDefinedBy <https://www.iso.org/standard/68078.html> ;
  rdfs:label "InformationContainer" ;
  rdfs:seeAlso bpmn:DataObject ;
  rdfs:subClassOf owl:Thing ;
  rdfs:subClassOf prov:Entity ;
  rdfs:subClassOf [
      rdf:type owl:Restriction ;
      owl:cardinality "1"^^xsd:nonNegativeInteger ;
      owl:onProperty idpo:derivedFromBPMN ;
    ] ;
  rdfs:subClassOf [
      rdf:type owl:Restriction ;
      owl:cardinality "1"^^xsd:nonNegativeInteger ;
      owl:onProperty idpo:hasStatus ;
    ] ;
  rdfs:subClassOf [
      rdf:type owl:Restriction ;
      owl:minCardinality "1"^^xsd:nonNegativeInteger ;
      owl:onProperty idpo:contains ;
    ] ;
  rdfs:subClassOf [
      rdf:type owl:Restriction ;
      owl:minCardinality "1"^^xsd:nonNegativeInteger ;
      owl:onProperty idpo:hasRequirement ;
    ] ;
  owl:equivalentClass ct:ContainerDescription ;
.
idpo:InformationDelivery
  rdf:type owl:Class ;
  rdfs:comment "This class is used to represent the activity of generation information regarding defined information requirements and delivery specifications. Instances of this class can be derived from bpmn2:Task individuals. This class is a subClass of prov:Activity which allows to associate additional provenance information." ;
  rdfs:label "InformationDelivery" ;
  rdfs:seeAlso bpmn:Activity ;
  rdfs:subClassOf owl:Thing ;
  rdfs:subClassOf prov:Activity ;
  rdfs:subClassOf [
      rdf:type owl:Restriction ;
      owl:cardinality "1"^^xsd:nonNegativeInteger ;
      owl:onProperty idpo:derivedFromBPMN ;
    ] ;
  rdfs:subClassOf [
      rdf:type owl:Restriction ;
      owl:cardinality "1"^^xsd:nonNegativeInteger ;
      owl:onProperty idpo:provides ;
    ] ;
.
idpo:InformationProvider
  rdf:type rdfs:Class ;
  rdfs:comment "ISO 19650-4 3.2.1 information provider: actor who provides information in an information container according to the requirements. Is equivalent to idpo:AppointedParty." ;
  rdfs:isDefinedBy <https://www.iso.org/standard/78246.html> ;
  rdfs:label "InformationProvider" ;
  rdfs:subClassOf idpo:Actor ;
  owl:equivalentClass idpo:AppointedParty ;
  skos:example "  A maintenance team will prepare an inspection report on an asset during an operational event." ;
  skos:example "  A structural engineer will prepare a detailed proposal during a detailed design stage." ;
.
idpo:InformationReceipt
  rdf:type owl:Class ;
  rdfs:comment "This class is used to represent the activity of using information regarding defined information requirements and delivery specifications. Instances of this class can be derived from bpmn2:Task individuals. This class is a subClass of prov:Activity which allows to associate additional provenance information." ;
  rdfs:label "InformationReceipt" ;
  rdfs:seeAlso bpmn:Activity ;
  rdfs:subClassOf owl:Thing ;
  rdfs:subClassOf prov:Activity ;
  rdfs:subClassOf [
      rdf:type owl:Restriction ;
      owl:cardinality "1"^^xsd:nonNegativeInteger ;
      owl:onProperty idpo:derivedFromBPMN ;
    ] ;
  rdfs:subClassOf [
      rdf:type owl:Restriction ;
      owl:cardinality "1"^^xsd:nonNegativeInteger ;
      owl:onProperty idpo:receives ;
    ] ;
.
idpo:InformationReceiver
  rdf:type rdfs:Class ;
  rdfs:comment "ISO 19650-4 3.2.2 information receiver: actor who receives information in an information container. Is equivalent to idpo:AppointingParty." ;
  rdfs:isDefinedBy <https://www.iso.org/standard/78246.html> ;
  rdfs:label "InformationReceiver" ;
  rdfs:subClassOf idpo:Actor ;
  owl:equivalentClass idpo:AppointingParty ;
.
idpo:PrefixDeclaration
  rdf:type sh:PrefixDeclaration ;
  sh:namespace "http://w3id.org/idpo#"^^xsd:anyURI ;
  sh:prefix "idpo" ;
.
idpo:Project
  rdf:type owl:Class ;
  rdfs:comment "This class represents a project and hosts the activities for generating and using information and the related persons." ;
  rdfs:label "Project" ;
  rdfs:subClassOf owl:Thing ;
  rdfs:subClassOf [
      rdf:type owl:Restriction ;
      owl:minCardinality "1"^^xsd:nonNegativeInteger ;
      owl:onProperty idpo:hasMember ;
    ] ;
  skos:prefLabel "Project" ;
.
idpo:Status
  rdf:type owl:Class ;
  rdfs:comment "This class represents the status of information." ;
  rdfs:label "Status" ;
  rdfs:subClassOf owl:Thing ;
  rdfs:subClassOf [
      rdf:type owl:Restriction ;
      owl:cardinality "1"^^xsd:nonNegativeInteger ;
      owl:onProperty idpo:status ;
    ] ;
  rdfs:subClassOf [
      rdf:type owl:Restriction ;
      owl:maxCardinality "1"^^xsd:nonNegativeInteger ;
      owl:onProperty idpo:statusSystem ;
    ] ;
.
idpo:appointsUsage
  rdf:type owl:ObjectProperty ;
  rdfs:comment "Associates an idpo:AppointingParty to a information Receipt" ;
  rdfs:domain idpo:AppointingParty ;
  rdfs:label "appointsUsage" ;
  rdfs:range idpo:InformationReceipt ;
  rdfs:subPropertyOf owl:topObjectProperty ;
  skos:prefLabel "appointsUsage" ;
.
idpo:belongsTo
  rdf:type owl:ObjectProperty ;
  rdfs:comment "Represents the usage of an information inside a project" ;
  rdfs:domain idpo:InformationDelivery ;
  rdfs:domain idpo:InformationReceipt ;
  rdfs:label "belongsTo" ;
  rdfs:range idpo:Project ;
  rdfs:subPropertyOf owl:topObjectProperty ;
.
idpo:contains
  rdf:type owl:ObjectProperty ;
  rdfs:comment "Associates any kind of data to an information container" ;
  rdfs:domain idpo:InformationContainer ;
  rdfs:label "contains" ;
  rdfs:range rdfs:Resource ;
  rdfs:subPropertyOf owl:topObjectProperty ;
.
idpo:defines
  rdf:type owl:ObjectProperty ;
  rdfs:domain idpo:AppointingParty ;
  rdfs:label "defines" ;
  rdfs:range idpo:ExchangeInformationRequirement ;
  owl:inverseOf idpo:isDefinedBy ;
  skos:prefLabel "defines" ;
.
idpo:derivedFromBPMN
  rdf:type owl:ObjectProperty ;
  rdfs:comment "Associates the BPMN object from which this individual has been derived" ;
  rdfs:domain idpo:InformationContainer ;
  rdfs:domain idpo:InformationDelivery ;
  rdfs:domain idpo:InformationReceipt ;
  rdfs:label "derivedFromBPMN" ;
  rdfs:range bpmn:Activity ;
  rdfs:range bpmn:DataObject ;
  rdfs:subPropertyOf owl:topObjectProperty ;
.
idpo:dueDate
  rdf:type owl:DatatypeProperty ;
  rdfs:comment "The due date of an information requirement" ;
  rdfs:domain idpo:ExchangeInformationRequirement ;
  rdfs:label "dueDate" ;
  rdfs:range xsd:dateTime ;
  rdfs:subPropertyOf owl:topDataProperty ;
.
idpo:hasInformationConstraint
  rdf:type owl:ObjectProperty ;
  rdfs:comment "ISO 29481-1 3.5 information constraint: statement that formally defines or constrains the scope of a piece of information due to some aspect of the business, a rule under which an organisation operates or a policy or decision that influences a process. Represents the concrete specification of delivered information as a sh:NodeShape." ;
  rdfs:domain idpo:ExchangeInformationRequirement ;
  rdfs:isDefinedBy <https://www.iso.org/standard/60553.html> ;
  rdfs:label "hasInformationConstraint" ;
  rdfs:range sh:NodeShape ;
  rdfs:subPropertyOf owl:topObjectProperty ;
.
idpo:hasMember
  rdf:type owl:ObjectProperty ;
  rdfs:comment "Associates a idpo:Actor to a project" ;
  rdfs:domain idpo:Project ;
  rdfs:label "hasMember" ;
  rdfs:range idpo:Actor ;
  rdfs:subPropertyOf owl:topObjectProperty ;
  owl:inverseOf idpo:isMemberOf ;
  skos:prefLabel "hasMember" ;
.
idpo:hasRequirement
  rdf:type owl:ObjectProperty ;
  rdfs:comment "Associates a requirement to an information" ;
  rdfs:domain idpo:InformationContainer ;
  rdfs:label "hasRequirement" ;
  rdfs:range idpo:ExchangeInformationRequirement ;
  rdfs:subPropertyOf owl:topObjectProperty ;
  owl:inverseOf idpo:isRequirementOf ;
.
idpo:hasStatus
  rdf:type owl:ObjectProperty ;
  rdfs:comment "Associates a status to an information" ;
  rdfs:domain idpo:InformationContainer ;
  rdfs:label "hasStatus" ;
  rdfs:range idpo:Status ;
  rdfs:subPropertyOf owl:topObjectProperty ;
  owl:inverseOf idpo:isStatusOf ;
  skos:prefLabel "hasStatus" ;
.
idpo:isAppointedForDelivery
  rdf:type owl:ObjectProperty ;
  rdfs:comment "Associates an idpo:AppointedParty to an idpo:InformationDelivery" ;
  rdfs:domain idpo:AppointedParty ;
  rdfs:label "isAppointedForDelivery" ;
  rdfs:range idpo:InformationDelivery ;
  rdfs:subPropertyOf owl:topObjectProperty ;
  skos:prefLabel "isAppointedForDelivery" ;
.
idpo:isDefinedBy
  rdf:type owl:ObjectProperty ;
  rdfs:domain idpo:ExchangeInformationRequirement ;
  rdfs:label "isDefinedBy" ;
  rdfs:range idpo:AppointingParty ;
  owl:inverseOf idpo:defines ;
  skos:prefLabel "isDefinedBy" ;
.
idpo:isMemberOf
  rdf:type owl:ObjectProperty ;
  rdfs:comment "Associates a project to an idpo:Actor" ;
  rdfs:domain idpo:Actor ;
  rdfs:label "isMemberOf" ;
  rdfs:range idpo:Project ;
  rdfs:subPropertyOf owl:topObjectProperty ;
  owl:inverseOf idpo:hasMember ;
  skos:prefLabel "isMemberOf" ;
.
idpo:isProvidedBy
  rdf:type owl:ObjectProperty ;
  rdfs:comment "Associates the originating information delivery to an information container. Inverse of idpo:provides." ;
  rdfs:domain idpo:InformationContainer ;
  rdfs:label "isProvidedBy" ;
  rdfs:range idpo:InformationDelivery ;
  rdfs:subPropertyOf owl:topObjectProperty ;
  rdfs:subPropertyOf prov:wasGeneratedBy ;
  owl:inverseOf idpo:provides ;
.
idpo:isReceivedBy
  rdf:type owl:ObjectProperty ;
  rdfs:comment "Represents the reception of an information container. Inverse of idpo:receives." ;
  rdfs:domain idpo:InformationContainer ;
  rdfs:label "isReceivedBy" ;
  rdfs:range idpo:InformationReceipt ;
  rdfs:subPropertyOf owl:topObjectProperty ;
  owl:inverseOf idpo:receives ;
  owl:propertyDisjointWith idpo:provides ;
.
idpo:isRequirementOf
  rdf:type owl:ObjectProperty ;
  rdfs:comment "Associates the originating information to a requirement" ;
  rdfs:domain idpo:ExchangeInformationRequirement ;
  rdfs:label "isRequirementOf" ;
  rdfs:range idpo:InformationContainer ;
  rdfs:subPropertyOf owl:topObjectProperty ;
  owl:inverseOf idpo:hasRequirement ;
  skos:prefLabel "isRequirementOf" ;
.
idpo:isStatusOf
  rdf:type owl:ObjectProperty ;
  rdfs:comment "Associates the information that uses a status" ;
  rdfs:domain idpo:Status ;
  rdfs:label "isStatusOf" ;
  rdfs:range idpo:InformationContainer ;
  rdfs:subPropertyOf owl:topObjectProperty ;
  owl:inverseOf idpo:hasStatus ;
  skos:prefLabel "isStatusOf" ;
.
idpo:priority
  rdf:type owl:DatatypeProperty ;
  rdfs:comment "Represents the priority of an information requirement, e. g. high, low, none" ;
  rdfs:domain idpo:ExchangeInformationRequirement ;
  rdfs:label "priority" ;
  rdfs:range xsd:string ;
  rdfs:subPropertyOf owl:topDataProperty ;
.
idpo:provides
  rdf:type owl:ObjectProperty ;
  rdfs:comment "Associates provided information containers to an information delivery. Inverse of idpo:isProvidedBy." ;
  rdfs:domain idpo:InformationDelivery ;
  rdfs:label "provides" ;
  rdfs:range idpo:InformationContainer ;
  rdfs:subPropertyOf owl:topObjectProperty ;
  rdfs:subPropertyOf prov:generated ;
  owl:inverseOf idpo:isProvidedBy ;
  owl:propertyDisjointWith idpo:receives ;
.
idpo:receives
  rdf:type owl:ObjectProperty ;
  rdfs:comment "Associates an received information container to an information receipt. Inverse of idpo:isReceivedBy" ;
  rdfs:domain idpo:InformationReceipt ;
  rdfs:label "receives" ;
  rdfs:range idpo:InformationContainer ;
  rdfs:subPropertyOf owl:topObjectProperty ;
  rdfs:subPropertyOf prov:used ;
  owl:inverseOf idpo:isReceivedBy ;
  owl:propertyDisjointWith idpo:provides ;
.
idpo:requires
  rdf:type owl:ObjectProperty ;
  rdfs:comment "Represents the concrete requirement of delivered information as a sh:NodeShape oder any other rdfs:Resource on the dataset and/or document level" ;
  rdfs:domain idpo:ExchangeInformationRequirement ;
  rdfs:label "requires" ;
  rdfs:range sh:Shape ;
  rdfs:subPropertyOf owl:topObjectProperty ;
.
idpo:status
  rdf:type owl:DatatypeProperty ;
  rdfs:comment "Represents the status string of a status individual, e. g. Work in Progess, Shared, Published, Archived" ;
  rdfs:domain idpo:Status ;
  rdfs:label "status" ;
  rdfs:range xsd:string ;
  rdfs:subPropertyOf owl:topDataProperty ;
.
idpo:statusSystem
  rdf:type owl:DatatypeProperty ;
  rdfs:comment "Represents the status system string of a status individual, e. g. ISO19650 or an URI to the originating status system" ;
  rdfs:domain idpo:Status ;
  rdfs:label "statusSystem" ;
  rdfs:range [
      rdf:type owl:Class ;
      owl:unionOf (
          xsd:string
          xsd:anyURI
        ) ;
    ] ;
  rdfs:subPropertyOf owl:topDataProperty ;
.
idpo:suitability
  rdf:type owl:DatatypeProperty ;
  rdfs:comment "Represents the suitability of information within an information requirement, e. g. regarding to ISO19650" ;
  rdfs:domain idpo:ExchangeInformationRequirement ;
  rdfs:label "suitablity" ;
  rdfs:range xsd:string ;
  rdfs:subPropertyOf owl:topDataProperty ;
.
bpmn:PrefixDeclaration
  rdf:type sh:PrefixDeclaration ;
  sh:namespace "http://www.omg.org/spec/BPMN/20100524/MODEL#"^^xsd:anyURI ;
  sh:prefix "bpmn2" ;
.
