# baseURI: https://w3id.org/dano
# prefix: dano

@prefix dano: <https://w3id.org/dano#> .
@prefix dc: <http://purl.org/dc/terms/> .
@prefix foaf: <http://xmlns.com/foaf/0.1/> .
@prefix geo: <http://www.opengis.net/ont/geosparql#> .
@prefix owl: <http://www.w3.org/2002/07/owl#> .
@prefix rdf: <http://www.w3.org/1999/02/22-rdf-syntax-ns#> .
@prefix rdfs: <http://www.w3.org/2000/01/rdf-schema#> .
@prefix schema: <https://schema.org/> .
@prefix skos: <http://www.w3.org/2004/02/skos/core#> .
@prefix vann: <http://purl.org/vocab/vann/> .
@prefix xsd: <http://www.w3.org/2001/XMLSchema#> .

<http://purl.org/dc/elements/1.1/coverage>
  rdfs:comment "The spatial or temporal topic of the resource, the spatial applicability of the resource, or the jurisdiction under which the resource is relevant."@en ;
  rdfs:isDefinedBy <http://purl.org/dc/elements/1.1/> ;
  rdfs:label "Coverage"@en ;
.
<http://purl.org/dc/elements/1.1/format>
  rdfs:comment "The file format, physical medium, or dimensions of the resource."@en ;
  rdfs:isDefinedBy <http://purl.org/dc/elements/1.1/> ;
  rdfs:label "Format"@en ;
.
<http://purl.org/dc/elements/1.1/identifier>
  rdfs:comment "An unambiguous reference to the resource within a given context."@en ;
  rdfs:isDefinedBy <http://purl.org/dc/elements/1.1/> ;
  rdfs:label "Identifier"@en ;
.
<http://purl.org/dc/elements/1.1/language>
  rdfs:comment "A language of the resource."@en ;
  rdfs:isDefinedBy <http://purl.org/dc/elements/1.1/> ;
  rdfs:label "Language"@en ;
  rdfs:seeAlso <http://www.ietf.org/rfc/rfc4646.txt> ;
.
<http://purl.org/dc/elements/1.1/publisher>
  rdfs:comment "An entity responsible for making the resource available."@en ;
  rdfs:isDefinedBy <http://purl.org/dc/elements/1.1/> ;
  rdfs:label "Publisher"@en ;
.
<http://purl.org/dc/elements/1.1/relation>
  rdfs:comment "A related resource."@en ;
  rdfs:isDefinedBy <http://purl.org/dc/elements/1.1/> ;
  rdfs:label "Relation"@en ;
.
<http://purl.org/dc/elements/1.1/rights>
  rdfs:comment "Information about rights held in and over the resource."@en ;
  rdfs:isDefinedBy <http://purl.org/dc/elements/1.1/> ;
  rdfs:label "Rights"@en ;
.
<http://purl.org/dc/elements/1.1/source>
  rdfs:comment "A related resource from which the described resource is derived."@en ;
  rdfs:isDefinedBy <http://purl.org/dc/elements/1.1/> ;
  rdfs:label "Source"@en ;
.
<http://purl.org/dc/elements/1.1/subject>
  rdfs:comment "The topic of the resource."@en ;
  rdfs:isDefinedBy <http://purl.org/dc/elements/1.1/> ;
  rdfs:label "Subject"@en ;
.
<http://purl.org/dc/elements/1.1/title>
  rdfs:comment "A name given to the resource."@en ;
  rdfs:isDefinedBy <http://purl.org/dc/elements/1.1/> ;
  rdfs:label "Title"@en ;
.
<http://purl.org/dc/elements/1.1/type>
  rdfs:comment "The nature or genre of the resource."@en ;
  rdfs:isDefinedBy <http://purl.org/dc/elements/1.1/> ;
  rdfs:label "Type"@en ;
.
<http://www.opengis.net/ont/geosparql>
  <http://purl.org/dc/elements/1.1/source> <http://www.opengis.net/doc/IS/geosparql/1.0> ;
  <http://purl.org/dc/elements/1.1/source> "OGC GeoSPARQL – A Geographic Query Language for RDF Data OGC 11-052r5" ;
  <http://purl.org/dc/elements/1.1/title> "GeoSPARQL Ontology" ;
  rdfs:seeAlso <http://www.opengis.net/def/function/ogc-geosparql/1.0> ;
  rdfs:seeAlso <http://www.opengis.net/def/rule/ogc-geosparql/1.0> ;
  rdfs:seeAlso <http://www.opengis.net/doc/IS/geosparql/1.0> ;
  owl:versionIRI <http://www.opengis.net/ont/geosparql/1.0> ;
  owl:versionInfo "OGC GeoSPARQL 1.0" ;
.
geo:defaultGeometry
  rdf:type owl:ObjectProperty ;
  rdfs:comment """
      The default geometry to be used in spatial calculations.
      It is Usually the most detailed geometry.
    """@en ;
  rdfs:isDefinedBy <http://www.opengis.net/ont/geosparql> ;
  rdfs:isDefinedBy <http://www.opengis.net/spec/geosparql/1.0> ;
  rdfs:label "defaultGeometry"@en ;
  rdfs:subPropertyOf geo:hasGeometry ;
.
geo:hasGeometry
  rdf:type owl:ObjectProperty ;
  rdfs:comment """
      A spatial representation for a given feature.
    """@en ;
  rdfs:isDefinedBy <http://www.opengis.net/ont/geosparql> ;
  rdfs:isDefinedBy <http://www.opengis.net/spec/geosparql/1.0> ;
  rdfs:label "hasGeometry"@en ;
.
xsd:date
  rdf:type rdfs:Datatype ;
.
schema:codeRepository
  rdf:type owl:Thing ;
.
schema:domainIncludes
  rdf:type owl:AnnotationProperty ;
.
schema:rangeIncludes
  rdf:type owl:AnnotationProperty ;
.
<https://w3id.org/dano>
  rdf:type owl:Ontology ;
  dc:creator [
      rdf:type schema:Person ;
      schema:email <mailto:phillip.schoenfelder@rub.de> ;
      schema:identifier <https://orcid.org/0000-0002-8685-436X> ;
      schema:memberOf [
          schema:identifier <https://www.inf.bi.ruhr-uni-bochum.de/iib/lehrstuhl/mitarbeiter/phillip_schoenfelder.html.en> ;
          schema:name "Ruhr-Universität Bochum" ;
        ] ;
      schema:name "Phillip Schönfelder" ;
    ] ;
  dc:description """This ontology covers concepts of technical drawings from the perspective of computer vision-based drawing analysis to be used in collaborative settings or for post-processing. 
The preferred namespace prefix is `dano` for the namespace IRI [https://w3id.org/dano](https://w3id.org/dano)."""@en ;
  dc:issued "2025-03-11"^^xsd:date ;
  dc:license <https://creativecommons.org/licenses/by/4.0/> ;
  dc:modified "2025-07-15"^^xsd:date ;
  dc:publisher [
      rdf:type foaf:Organization ;
      foaf:homepage <http://www.inf.bi.rub.de> ;
      foaf:name "Chair of Computing in Engineering" ;
    ] ;
  dc:rights "Copyright 2025 by Phillip Schönfelder" ;
  dc:source <https://github.com/RUB-Informatik-im-Bauwesen/dano> ;
  dc:title "Drawing Analyis Ontology (DAnO)"@en ;
  vann:preferredNamespacePrefix "dano" ;
  vann:preferredNamespaceUri <https://w3id.org/dano> ;
  owl:versionIRI <https://w3id.org/dano> ;
  owl:versionInfo "v0.2" ;
  skos:historyNote """  
  v0.1: initial ontology
  
  v0.2: added cardinality constraints to the taxonomy, restructured taxonomy, modified image
 """ ;
.
dano:AxisLine
  rdf:type owl:Class ;
  rdfs:label "Axis Line" ;
  rdfs:subClassOf dano:Line ;
.
dano:Composite
  rdf:type owl:Class ;
  rdfs:comment "A composite element that aggregates multiple description elements." ;
  rdfs:label "Composite" ;
  rdfs:subClassOf dano:DescriptionElement ;
.
dano:DescriptionElement
  rdf:type owl:Class ;
  rdfs:comment "An abstract element in a drawing describing properties of display elements. For instance, a dimension line describing a wall or a text element specifying a schematic pump symbol." ;
  rdfs:label "Description Element" ;
  rdfs:subClassOf dano:DrawingElement ;
.
dano:Dimension
  rdf:type owl:Class ;
  rdfs:comment "A composite element, comprising exactly 1 DimensionLine, 2 Terminators (at the line's ends), and 1 TextElement (for the dimension value)." ;
  rdfs:label "Dimension" ;
  rdfs:subClassOf dano:Composite ;
  rdfs:subClassOf [
      rdf:type owl:Restriction ;
      owl:onClass dano:DimensionLine ;
      owl:onProperty dano:contains ;
      owl:qualifiedCardinality "1"^^xsd:nonNegativeInteger ;
    ] ;
  rdfs:subClassOf [
      rdf:type owl:Restriction ;
      owl:onClass dano:Terminator ;
      owl:onProperty dano:contains ;
      owl:qualifiedCardinality "2"^^xsd:nonNegativeInteger ;
    ] ;
  rdfs:subClassOf [
      rdf:type owl:Restriction ;
      owl:onClass dano:TextElement ;
      owl:onProperty dano:contains ;
      owl:qualifiedCardinality "1"^^xsd:nonNegativeInteger ;
    ] ;
.
dano:DimensionChain
  rdf:type owl:Class ;
  rdfs:comment "A sequence of dimensions connected together to represent cumulative measurements." ;
  rdfs:label "Dimension Chain" ;
  rdfs:subClassOf dano:Composite ;
  rdfs:subClassOf [
      rdf:type owl:Restriction ;
      owl:minQualifiedCardinality "2"^^xsd:nonNegativeInteger ;
      owl:onClass dano:Dimension ;
      owl:onProperty dano:contains ;
    ] ;
.
dano:DimensionLine
  rdf:type owl:Class ;
  rdfs:comment "The line type for indicating dimensions in a drawing, typically used to represent measurements." ;
  rdfs:label "Dimension Line" ;
  rdfs:subClassOf dano:Line ;
.
dano:Dimension_1
  rdf:type dano:Dimension ;
  rdfs:label "Dimension" ;
.
dano:DisplayElement
  rdf:type owl:Class ;
  rdfs:comment "An element representing a real-world component." ;
  rdfs:label "Display Element" ;
  rdfs:subClassOf dano:DrawingElement ;
.
dano:DrawingElement
  rdf:type owl:Class ;
  rdfs:comment "A visual element in a drawing. Metadata for these elements are stored as DrawingElementMeta instances." ;
  rdfs:label "Drawing Element" ;
  rdfs:subClassOf owl:Thing ;
.
dano:DrawingElementMeta
  rdf:type owl:Class ;
  rdfs:comment "Metadata for drawing elements, including inference confidence and methods used." ;
  rdfs:label "Drawing Element Meta" ;
  rdfs:subClassOf owl:Thing ;
.
dano:EquipmentSymbol
  rdf:type owl:Class ;
  rdfs:label "Equipment symbol" ;
  rdfs:subClassOf dano:Symbol ;
.
dano:Line
  rdf:type owl:Class ;
  rdfs:comment "A linear description element in a drawing." ;
  rdfs:label "Line" ;
  rdfs:subClassOf dano:DescriptionElement ;
.
dano:SectionSymbol
  rdf:type owl:Class ;
  rdfs:comment "A symbol defining the section plane that opens up a view section. Must have a partner symbol and is referred to by a TextElement which is its reference letter." ;
  rdfs:label "Section Symbol" ;
  rdfs:subClassOf dano:Symbol ;
.
dano:Symbol
  rdf:type owl:Class ;
  rdfs:comment "A symbolic description element representing various annotations or markers." ;
  rdfs:label "Symbol" ;
  rdfs:subClassOf dano:DescriptionElement ;
.
dano:Terminator
  rdf:type owl:Class ;
  rdfs:comment "A marker used to indicate endpoints or reference points on a dimension line." ;
  rdfs:label "Terminator" ;
  rdfs:subClassOf dano:Symbol ;
.
dano:TextElement
  rdf:type owl:Class ;
  rdfs:comment "A text-based description element in a drawing." ;
  rdfs:label "Text Element" ;
  rdfs:subClassOf dano:DescriptionElement ;
.
dano:TextField
  rdf:type owl:Class ;
  rdfs:comment "A composite element containing multiple text elements, typically for multiline text." ;
  rdfs:label "Text Field" ;
  rdfs:subClassOf dano:Composite ;
  rdfs:subClassOf [
      rdf:type owl:Restriction ;
      owl:minQualifiedCardinality "2"^^xsd:nonNegativeInteger ;
      owl:onClass dano:TextElement ;
      owl:onProperty dano:contains ;
    ] ;
.
dano:contains
  rdf:type owl:ObjectProperty ;
  rdf:type owl:TransitiveProperty ;
  rdfs:comment "Indicates that the subject drawing element contains the object drawing element. For instance, lines can contain two endpoints." ;
  rdfs:domain dano:DrawingElement ;
  rdfs:label "contains" ;
  rdfs:range dano:DrawingElement ;
  owl:inverseOf dano:isContainedIn ;
.
dano:depicts
  rdf:type owl:ObjectProperty ;
  rdfs:comment "Indicates that the subject display element graphically represents a real-world object, such as a building element, zone, or machine part." ;
  rdfs:domain dano:DisplayElement ;
  rdfs:label "depicts" ;
.
dano:describes
  rdf:type owl:ObjectProperty ;
  rdfs:comment "Establishes the relationship between a description element and a display element, where the description element describes the display element." ;
  rdfs:domain dano:DescriptionElement ;
  rdfs:label "describes" ;
  rdfs:range dano:DisplayElement ;
  owl:inverseOf dano:isDescribedBy ;
.
dano:endsWith
  rdf:type owl:ObjectProperty ;
  rdfs:comment "Indicates that a dimension line ends with a dimension line marker." ;
  rdfs:domain dano:DimensionLine ;
  rdfs:label "ends with" ;
  rdfs:range dano:Terminator ;
  rdfs:subPropertyOf dano:contains ;
.
dano:hasConfidence
  rdf:type owl:DatatypeProperty ;
  rdfs:comment "Specifies the confidence level of the inference that identified the drawing element." ;
  rdfs:domain dano:DrawingElement ;
  rdfs:label "has confidence" ;
  rdfs:range xsd:decimal ;
.
dano:hasGeometry
  rdf:type owl:ObjectProperty ;
  rdfs:comment "Links the drawing element to its geometrical representation." ;
  rdfs:domain dano:DrawingElement ;
  rdfs:label "has geometry" ;
.
dano:hasIfcRepresentation
  rdf:type owl:DatatypeProperty ;
  rdfs:comment "Specifies the IFC representation of the drawing element." ;
  rdfs:domain dano:DrawingElement ;
  rdfs:label "has IFC representation" ;
.
dano:hasMeta
  rdf:type owl:ObjectProperty ;
  rdfs:comment "Links meta information to a drawing element." ;
  rdfs:domain dano:DrawingElement ;
  rdfs:label "has meta" ;
  rdfs:range dano:DrawingElementMeta ;
.
dano:inferredAt
  rdf:type owl:DatatypeProperty ;
  rdfs:comment "Specifies the date when the drawing element was inferred." ;
  rdfs:domain dano:DrawingElementMeta ;
  rdfs:label "inferred at" ;
  rdfs:range xsd:date ;
.
dano:inferredBy
  rdf:type owl:DatatypeProperty ;
  rdfs:comment "Indicates the actor, company, or software that inferred the drawing element." ;
  rdfs:domain dano:DrawingElementMeta ;
  rdfs:label "inferred by" ;
  rdfs:range xsd:string ;
.
dano:inferredFrom
  rdf:type owl:DatatypeProperty ;
  rdfs:comment "Specifies the origin file from which the drawing element was extracted." ;
  rdfs:domain dano:DrawingElementMeta ;
  rdfs:label "inferred from" ;
  rdfs:range xsd:string ;
.
dano:inferredWith
  rdf:type owl:DatatypeProperty ;
  rdfs:comment "Indicates the algorithm used to infer the drawing element." ;
  rdfs:domain dano:DrawingElementMeta ;
  rdfs:label "inferred with" ;
  rdfs:range xsd:string ;
.
dano:isContainedIn
  rdf:type owl:ObjectProperty ;
  rdfs:comment "Indicates that the subject drawing element is part of another drawing element." ;
  rdfs:domain dano:DrawingElement ;
  rdfs:label "is contained in" ;
  rdfs:range dano:DrawingElement ;
  owl:inverseOf dano:contains ;
.
dano:isDepictedBy
  rdf:type owl:ObjectProperty ;
  rdfs:comment "Indicates that the real-world subject is depicted by the object display element, which is typically a geometric representation." ;
  rdfs:label "isDepictedBy" ;
  rdfs:range dano:DisplayElement ;
  owl:inverseOf dano:depicts ;
.
dano:isDescribedBy
  rdf:type owl:ObjectProperty ;
  rdfs:comment "Indicates that the display element is described by a description element." ;
  rdfs:domain dano:DisplayElement ;
  rdfs:label "is described by" ;
  rdfs:range dano:DescriptionElement ;
  owl:inverseOf dano:describes ;
.
dano:isReferredToBy
  rdf:type owl:ObjectProperty ;
  rdfs:comment "Indicates that the subject dimension line marker is referred to by another dimension line marker." ;
  rdfs:domain dano:Terminator ;
  rdfs:label "is referred to by" ;
  rdfs:range dano:Terminator ;
  owl:inverseOf dano:refersTo ;
.
dano:isText
  rdf:type owl:DatatypeProperty ;
  rdfs:comment "Indicates that the description element is a text element containing the specified string." ;
  rdfs:domain dano:TextElement ;
  rdfs:label "is text" ;
  rdfs:range xsd:string ;
.
dano:refersTo
  rdf:type owl:ObjectProperty ;
  rdfs:comment "Indicates that the subject dimension line marker refers to another dimension line marker." ;
  rdfs:domain dano:Terminator ;
  rdfs:label "refers to" ;
  rdfs:range dano:Terminator ;
  owl:inverseOf dano:isReferredToBy ;
.
